pulse/src/ocaml/plugin/generated/Pulse_Checker_Rewrite.ml
@@ -1,1 +1,580 @@
 open Prims
+let (check_rewrite :
+  Pulse_Typing_Env.env ->
+    Pulse_Syntax_Base.st_term ->
+      Pulse_Syntax_Base.term ->
+        unit ->
+          unit Pulse_Typing.post_hint_opt ->
+            ((unit, unit, unit) Pulse_Checker_Common.checker_result_t, 
+              unit) FStar_Tactics_Effect.tac_repr)
+  =
+  fun g ->
+    fun t ->
+      fun pre ->
+        fun pre_typing ->
+          fun post_hint ->
+            FStar_Tactics_Effect.tac_bind
+              (FStar_Sealed.seal
+                 (Obj.magic
+                    (FStar_Range.mk_range "Pulse.Checker.Rewrite.fst"
+                       (Prims.of_int (23)) (Prims.of_int (10))
+                       (Prims.of_int (23)) (Prims.of_int (48)))))
+              (FStar_Sealed.seal
+                 (Obj.magic
+                    (FStar_Range.mk_range "Pulse.Checker.Rewrite.fst"
+                       (Prims.of_int (23)) (Prims.of_int (51))
+                       (Prims.of_int (45)) (Prims.of_int (54)))))
+              (FStar_Tactics_Effect.lift_div_tac
+                 (fun uu___ ->
+                    Pulse_Checker_Pure.push_context "check_rewrite"
+                      t.Pulse_Syntax_Base.range2 g))
+              (fun uu___ ->
+                 (fun g1 ->
+                    Obj.magic
+                      (FStar_Tactics_Effect.tac_bind
+                         (FStar_Sealed.seal
+                            (Obj.magic
+                               (FStar_Range.mk_range
+                                  "Pulse.Checker.Rewrite.fst"
+                                  (Prims.of_int (24)) (Prims.of_int (32))
+                                  (Prims.of_int (24)) (Prims.of_int (38)))))
+                         (FStar_Sealed.seal
+                            (Obj.magic
+                               (FStar_Range.mk_range
+                                  "Pulse.Checker.Rewrite.fst"
+                                  (Prims.of_int (23)) (Prims.of_int (51))
+                                  (Prims.of_int (45)) (Prims.of_int (54)))))
+                         (FStar_Tactics_Effect.lift_div_tac
+                            (fun uu___ -> t.Pulse_Syntax_Base.term1))
+                         (fun uu___ ->
+                            (fun uu___ ->
+                               match uu___ with
+                               | Pulse_Syntax_Base.Tm_Rewrite
+                                   { Pulse_Syntax_Base.t1 = p;
+                                     Pulse_Syntax_Base.t2 = q;_}
+                                   ->
+                                   Obj.magic
+                                     (FStar_Tactics_Effect.tac_bind
+                                        (FStar_Sealed.seal
+                                           (Obj.magic
+                                              (FStar_Range.mk_range
+                                                 "Pulse.Checker.Rewrite.fst"
+                                                 (Prims.of_int (25))
+                                                 (Prims.of_int (26))
+                                                 (Prims.of_int (25))
+                                                 (Prims.of_int (41)))))
+                                        (FStar_Sealed.seal
+                                           (Obj.magic
+                                              (FStar_Range.mk_range
+                                                 "Pulse.Checker.Rewrite.fst"
+                                                 (Prims.of_int (24))
+                                                 (Prims.of_int (41))
+                                                 (Prims.of_int (45))
+                                                 (Prims.of_int (54)))))
+                                        (Obj.magic
+                                           (Pulse_Checker_Pure.check_vprop g1
+                                              p))
+                                        (fun uu___1 ->
+                                           (fun uu___1 ->
+                                              match uu___1 with
+                                              | Prims.Mkdtuple2
+                                                  (p1, p_typing) ->
+                                                  Obj.magic
+                                                    (FStar_Tactics_Effect.tac_bind
+                                                       (FStar_Sealed.seal
+                                                          (Obj.magic
+                                                             (FStar_Range.mk_range
+                                                                "Pulse.Checker.Rewrite.fst"
+                                                                (Prims.of_int (26))
+                                                                (Prims.of_int (26))
+                                                                (Prims.of_int (26))
+                                                                (Prims.of_int (41)))))
+                                                       (FStar_Sealed.seal
+                                                          (Obj.magic
+                                                             (FStar_Range.mk_range
+                                                                "Pulse.Checker.Rewrite.fst"
+                                                                (Prims.of_int (25))
+                                                                (Prims.of_int (44))
+                                                                (Prims.of_int (45))
+                                                                (Prims.of_int (54)))))
+                                                       (Obj.magic
+                                                          (Pulse_Checker_Pure.check_vprop
+                                                             g1 q))
+                                                       (fun uu___2 ->
+                                                          (fun uu___2 ->
+                                                             match uu___2
+                                                             with
+                                                             | Prims.Mkdtuple2
+                                                                 (q1,
+                                                                  q_typing)
+                                                                 ->
+                                                                 Obj.magic
+                                                                   (FStar_Tactics_Effect.tac_bind
+                                                                    (FStar_Sealed.seal
+                                                                    (Obj.magic
+                                                                    (FStar_Range.mk_range
+                                                                    "Pulse.Checker.Rewrite.fst"
+                                                                    (Prims.of_int (28))
+                                                                    (Prims.of_int (6))
+                                                                    (Prims.of_int (43))
+                                                                    (Prims.of_int (30)))))
+                                                                    (FStar_Sealed.seal
+                                                                    (Obj.magic
+                                                                    (FStar_Range.mk_range
+                                                                    "Pulse.Checker.Rewrite.fst"
+                                                                    (Prims.of_int (43))
+                                                                    (Prims.of_int (33))
+                                                                    (Prims.of_int (45))
+                                                                    (Prims.of_int (54)))))
+                                                                    (if
+                                                                    Pulse_Syntax_Base.eq_tm
+                                                                    p1 q1
+                                                                    then
+                                                                    Obj.magic
+                                                                    (Obj.repr
+                                                                    (FStar_Tactics_Effect.lift_div_tac
+                                                                    (fun
+                                                                    uu___3 ->
+                                                                    ())))
+                                                                    else
+                                                                    Obj.magic
+                                                                    (Obj.repr
+                                                                    (FStar_Tactics_Effect.tac_bind
+                                                                    (FStar_Sealed.seal
+                                                                    (Obj.magic
+                                                                    (FStar_Range.mk_range
+                                                                    "Pulse.Checker.Rewrite.fst"
+                                                                    (Prims.of_int (30))
+                                                                    (Prims.of_int (24))
+                                                                    (Prims.of_int (30))
+                                                                    (Prims.of_int (35)))))
+                                                                    (FStar_Sealed.seal
+                                                                    (Obj.magic
+                                                                    (FStar_Range.mk_range
+                                                                    "Pulse.Checker.Rewrite.fst"
+                                                                    (Prims.of_int (30))
+                                                                    (Prims.of_int (38))
+                                                                    (Prims.of_int (43))
+                                                                    (Prims.of_int (30)))))
+                                                                    (FStar_Tactics_Effect.lift_div_tac
+                                                                    (fun
+                                                                    uu___4 ->
+                                                                    Pulse_Elaborate_Pure.elab_term
+                                                                    p1))
+                                                                    (fun
+                                                                    uu___4 ->
+                                                                    (fun
+                                                                    elab_p ->
+                                                                    Obj.magic
+                                                                    (FStar_Tactics_Effect.tac_bind
+                                                                    (FStar_Sealed.seal
+                                                                    (Obj.magic
+                                                                    (FStar_Range.mk_range
+                                                                    "Pulse.Checker.Rewrite.fst"
+                                                                    (Prims.of_int (31))
+                                                                    (Prims.of_int (24))
+                                                                    (Prims.of_int (31))
+                                                                    (Prims.of_int (35)))))
+                                                                    (FStar_Sealed.seal
+                                                                    (Obj.magic
+                                                                    (FStar_Range.mk_range
+                                                                    "Pulse.Checker.Rewrite.fst"
+                                                                    (Prims.of_int (31))
+                                                                    (Prims.of_int (38))
+                                                                    (Prims.of_int (43))
+                                                                    (Prims.of_int (30)))))
+                                                                    (FStar_Tactics_Effect.lift_div_tac
+                                                                    (fun
+                                                                    uu___4 ->
+                                                                    Pulse_Elaborate_Pure.elab_term
+                                                                    q1))
+                                                                    (fun
+                                                                    uu___4 ->
+                                                                    (fun
+                                                                    elab_q ->
+                                                                    Obj.magic
+                                                                    (FStar_Tactics_Effect.tac_bind
+                                                                    (FStar_Sealed.seal
+                                                                    (Obj.magic
+                                                                    (FStar_Range.mk_range
+                                                                    "Pulse.Checker.Rewrite.fst"
+                                                                    (Prims.of_int (32))
+                                                                    (Prims.of_int (29))
+                                                                    (Prims.of_int (32))
+                                                                    (Prims.of_int (69)))))
+                                                                    (FStar_Sealed.seal
+                                                                    (Obj.magic
+                                                                    (FStar_Range.mk_range
+                                                                    "Pulse.Checker.Rewrite.fst"
+                                                                    (Prims.of_int (31))
+                                                                    (Prims.of_int (38))
+                                                                    (Prims.of_int (43))
+                                                                    (Prims.of_int (30)))))
+                                                                    (Obj.magic
+                                                                    (FStar_Tactics_V2_Builtins.check_equiv
+                                                                    (Pulse_Typing.elab_env
+                                                                    g1)
+                                                                    elab_p
+                                                                    elab_q))
+                                                                    (fun
+                                                                    uu___4 ->
+                                                                    (fun
+                                                                    uu___4 ->
+                                                                    match uu___4
+                                                                    with
+                                                                    | 
+                                                                    (res,
+                                                                    issues)
+                                                                    ->
+                                                                    Obj.magic
+                                                                    (FStar_Tactics_Effect.tac_bind
+                                                                    (FStar_Sealed.seal
+                                                                    (Obj.magic
+                                                                    (FStar_Range.mk_range
+                                                                    "Pulse.Checker.Rewrite.fst"
+                                                                    (Prims.of_int (33))
+                                                                    (Prims.of_int (11))
+                                                                    (Prims.of_int (33))
+                                                                    (Prims.of_int (30)))))
+                                                                    (FStar_Sealed.seal
+                                                                    (Obj.magic
+                                                                    (FStar_Range.mk_range
+                                                                    "Pulse.Checker.Rewrite.fst"
+                                                                    (Prims.of_int (34))
+                                                                    (Prims.of_int (11))
+                                                                    (Prims.of_int (43))
+                                                                    (Prims.of_int (30)))))
+                                                                    (Obj.magic
+                                                                    (FStar_Tactics_V2_Builtins.log_issues
+                                                                    issues))
+                                                                    (fun
+                                                                    uu___5 ->
+                                                                    (fun
+                                                                    uu___5 ->
+                                                                    match res
+                                                                    with
+                                                                    | 
+                                                                    FStar_Pervasives_Native.None
+                                                                    ->
+                                                                    Obj.magic
+                                                                    (Obj.repr
+                                                                    (FStar_Tactics_Effect.tac_bind
+                                                                    (FStar_Sealed.seal
+                                                                    (Obj.magic
+                                                                    (FStar_Range.mk_range
+                                                                    "Pulse.Checker.Rewrite.fst"
+                                                                    (Prims.of_int (37))
+                                                                    (Prims.of_int (20))
+                                                                    (Prims.of_int (41))
+                                                                    (Prims.of_int (53)))))
+                                                                    (FStar_Sealed.seal
+                                                                    (Obj.magic
+                                                                    (FStar_Range.mk_range
+                                                                    "Pulse.Checker.Rewrite.fst"
+                                                                    (Prims.of_int (36))
+                                                                    (Prims.of_int (13))
+                                                                    (Prims.of_int (41))
+                                                                    (Prims.of_int (53)))))
+                                                                    (Obj.magic
+                                                                    (FStar_Tactics_Effect.tac_bind
+                                                                    (FStar_Sealed.seal
+                                                                    (Obj.magic
+                                                                    (FStar_Range.mk_range
+                                                                    "Pulse.Checker.Rewrite.fst"
+                                                                    (Prims.of_int (41))
+                                                                    (Prims.of_int (27))
+                                                                    (Prims.of_int (41))
+                                                                    (Prims.of_int (52)))))
+                                                                    (FStar_Sealed.seal
+                                                                    (Obj.magic
+                                                                    (FStar_Range.mk_range
+                                                                    "Pulse.Checker.Rewrite.fst"
+                                                                    (Prims.of_int (37))
+                                                                    (Prims.of_int (20))
+                                                                    (Prims.of_int (41))
+                                                                    (Prims.of_int (53)))))
+                                                                    (Obj.magic
+                                                                    (FStar_Tactics_V2_Builtins.term_to_string
+                                                                    elab_q))
+                                                                    (fun
+                                                                    uu___6 ->
+                                                                    (fun
+                                                                    uu___6 ->
+                                                                    Obj.magic
+                                                                    (FStar_Tactics_Effect.tac_bind
+                                                                    (FStar_Sealed.seal
+                                                                    (Obj.magic
+                                                                    (FStar_Range.mk_range
+                                                                    "Pulse.Checker.Rewrite.fst"
+                                                                    (Prims.of_int (37))
+                                                                    (Prims.of_int (20))
+                                                                    (Prims.of_int (41))
+                                                                    (Prims.of_int (53)))))
+                                                                    (FStar_Sealed.seal
+                                                                    (Obj.magic
+                                                                    (FStar_Range.mk_range
+                                                                    "Pulse.Checker.Rewrite.fst"
+                                                                    (Prims.of_int (37))
+                                                                    (Prims.of_int (20))
+                                                                    (Prims.of_int (41))
+                                                                    (Prims.of_int (53)))))
+                                                                    (Obj.magic
+                                                                    (FStar_Tactics_Effect.tac_bind
+                                                                    (FStar_Sealed.seal
+                                                                    (Obj.magic
+                                                                    (FStar_Range.mk_range
+                                                                    "Pulse.Checker.Rewrite.fst"
+                                                                    (Prims.of_int (40))
+                                                                    (Prims.of_int (27))
+                                                                    (Prims.of_int (40))
+                                                                    (Prims.of_int (52)))))
+                                                                    (FStar_Sealed.seal
+                                                                    (Obj.magic
+                                                                    (FStar_Range.mk_range
+                                                                    "Pulse.Checker.Rewrite.fst"
+                                                                    (Prims.of_int (37))
+                                                                    (Prims.of_int (20))
+                                                                    (Prims.of_int (41))
+                                                                    (Prims.of_int (53)))))
+                                                                    (Obj.magic
+                                                                    (FStar_Tactics_V2_Builtins.term_to_string
+                                                                    elab_p))
+                                                                    (fun
+                                                                    uu___7 ->
+                                                                    (fun
+                                                                    uu___7 ->
+                                                                    Obj.magic
+                                                                    (FStar_Tactics_Effect.tac_bind
+                                                                    (FStar_Sealed.seal
+                                                                    (Obj.magic
+                                                                    (FStar_Range.mk_range
+                                                                    "Pulse.Checker.Rewrite.fst"
+                                                                    (Prims.of_int (37))
+                                                                    (Prims.of_int (20))
+                                                                    (Prims.of_int (41))
+                                                                    (Prims.of_int (53)))))
+                                                                    (FStar_Sealed.seal
+                                                                    (Obj.magic
+                                                                    (FStar_Range.mk_range
+                                                                    "Pulse.Checker.Rewrite.fst"
+                                                                    (Prims.of_int (37))
+                                                                    (Prims.of_int (20))
+                                                                    (Prims.of_int (41))
+                                                                    (Prims.of_int (53)))))
+                                                                    (Obj.magic
+                                                                    (FStar_Tactics_Effect.tac_bind
+                                                                    (FStar_Sealed.seal
+                                                                    (Obj.magic
+                                                                    (FStar_Range.mk_range
+                                                                    "Pulse.Checker.Rewrite.fst"
+                                                                    (Prims.of_int (39))
+                                                                    (Prims.of_int (27))
+                                                                    (Prims.of_int (39))
+                                                                    (Prims.of_int (47)))))
+                                                                    (FStar_Sealed.seal
+                                                                    (Obj.magic
+                                                                    (FStar_Range.mk_range
+                                                                    "Pulse.Checker.Rewrite.fst"
+                                                                    (Prims.of_int (37))
+                                                                    (Prims.of_int (20))
+                                                                    (Prims.of_int (41))
+                                                                    (Prims.of_int (53)))))
+                                                                    (Obj.magic
+                                                                    (Pulse_Syntax_Printer.term_to_string
+                                                                    q1))
+                                                                    (fun
+                                                                    uu___8 ->
+                                                                    (fun
+                                                                    uu___8 ->
+                                                                    Obj.magic
+                                                                    (FStar_Tactics_Effect.tac_bind
+                                                                    (FStar_Sealed.seal
+                                                                    (Obj.magic
+                                                                    (FStar_Range.mk_range
+                                                                    "Pulse.Checker.Rewrite.fst"
+                                                                    (Prims.of_int (37))
+                                                                    (Prims.of_int (20))
+                                                                    (Prims.of_int (41))
+                                                                    (Prims.of_int (53)))))
+                                                                    (FStar_Sealed.seal
+                                                                    (Obj.magic
+                                                                    (FStar_Range.mk_range
+                                                                    "Pulse.Checker.Rewrite.fst"
+                                                                    (Prims.of_int (37))
+                                                                    (Prims.of_int (20))
+                                                                    (Prims.of_int (41))
+                                                                    (Prims.of_int (53)))))
+                                                                    (Obj.magic
+                                                                    (FStar_Tactics_Effect.tac_bind
+                                                                    (FStar_Sealed.seal
+                                                                    (Obj.magic
+                                                                    (FStar_Range.mk_range
+                                                                    "Pulse.Checker.Rewrite.fst"
+                                                                    (Prims.of_int (38))
+                                                                    (Prims.of_int (27))
+                                                                    (Prims.of_int (38))
+                                                                    (Prims.of_int (47)))))
+                                                                    (FStar_Sealed.seal
+                                                                    (Obj.magic
+                                                                    (FStar_Range.mk_range
+                                                                    "FStar.Printf.fst"
+                                                                    (Prims.of_int (121))
+                                                                    (Prims.of_int (8))
+                                                                    (Prims.of_int (123))
+                                                                    (Prims.of_int (44)))))
+                                                                    (Obj.magic
+                                                                    (Pulse_Syntax_Printer.term_to_string
+                                                                    p1))
+                                                                    (fun
+                                                                    uu___9 ->
+                                                                    FStar_Tactics_Effect.lift_div_tac
+                                                                    (fun
+                                                                    uu___10
+                                                                    ->
+                                                                    fun x ->
+                                                                    fun x1 ->
+                                                                    fun x2 ->
+                                                                    Prims.strcat
+                                                                    (Prims.strcat
+                                                                    (Prims.strcat
+                                                                    (Prims.strcat
+                                                                    "rewrite: could not prove equality of "
+                                                                    (Prims.strcat
+                                                                    uu___9
+                                                                    " and "))
+                                                                    (Prims.strcat
+                                                                    x
+                                                                    "\nElaborations: "))
+                                                                    (Prims.strcat
+                                                                    x1
+                                                                    " and "))
+                                                                    (Prims.strcat
+                                                                    x2 "\n")))))
+                                                                    (fun
+                                                                    uu___9 ->
+                                                                    FStar_Tactics_Effect.lift_div_tac
+                                                                    (fun
+                                                                    uu___10
+                                                                    ->
+                                                                    uu___9
+                                                                    uu___8))))
+                                                                    uu___8)))
+                                                                    (fun
+                                                                    uu___8 ->
+                                                                    FStar_Tactics_Effect.lift_div_tac
+                                                                    (fun
+                                                                    uu___9 ->
+                                                                    uu___8
+                                                                    uu___7))))
+                                                                    uu___7)))
+                                                                    (fun
+                                                                    uu___7 ->
+                                                                    FStar_Tactics_Effect.lift_div_tac
+                                                                    (fun
+                                                                    uu___8 ->
+                                                                    uu___7
+                                                                    uu___6))))
+                                                                    uu___6)))
+                                                                    (fun
+                                                                    uu___6 ->
+                                                                    (fun
+                                                                    uu___6 ->
+                                                                    Obj.magic
+                                                                    (Pulse_Typing_Env.fail
+                                                                    g1
+                                                                    (FStar_Pervasives_Native.Some
+                                                                    (t.Pulse_Syntax_Base.range2))
+                                                                    uu___6))
+                                                                    uu___6)))
+                                                                    | 
+                                                                    FStar_Pervasives_Native.Some
+                                                                    token ->
+                                                                    Obj.magic
+                                                                    (Obj.repr
+                                                                    (FStar_Tactics_Effect.lift_div_tac
+                                                                    (fun
+                                                                    uu___6 ->
+                                                                    ()))))
+                                                                    uu___5)))
+                                                                    uu___4)))
+                                                                    uu___4)))
+                                                                    uu___4))))
+                                                                    (fun
+                                                                    uu___3 ->
+                                                                    (fun
+                                                                    equiv_p_q
+                                                                    ->
+                                                                    Obj.magic
+                                                                    (FStar_Tactics_Effect.tac_bind
+                                                                    (FStar_Sealed.seal
+                                                                    (Obj.magic
+                                                                    (FStar_Range.mk_range
+                                                                    "Pulse.Checker.Rewrite.fst"
+                                                                    (Prims.of_int (44))
+                                                                    (Prims.of_int (9))
+                                                                    (Prims.of_int (44))
+                                                                    (Prims.of_int (43)))))
+                                                                    (FStar_Sealed.seal
+                                                                    (Obj.magic
+                                                                    (FStar_Range.mk_range
+                                                                    "Pulse.Checker.Rewrite.fst"
+                                                                    (Prims.of_int (45))
+                                                                    Prims.int_one
+                                                                    (Prims.of_int (45))
+                                                                    (Prims.of_int (54)))))
+                                                                    (FStar_Tactics_Effect.lift_div_tac
+                                                                    (fun
+                                                                    uu___3 ->
+                                                                    Pulse_Typing.T_Rewrite
+                                                                    (g1, p1,
+                                                                    q1, (),
+                                                                    ())))
+                                                                    (fun
+                                                                    uu___3 ->
+                                                                    (fun d ->
+                                                                    Obj.magic
+                                                                    (FStar_Tactics_Effect.tac_bind
+                                                                    (FStar_Sealed.seal
+                                                                    (Obj.magic
+                                                                    (FStar_Range.mk_range
+                                                                    "Pulse.Checker.Rewrite.fst"
+                                                                    (Prims.of_int (45))
+                                                                    (Prims.of_int (8))
+                                                                    (Prims.of_int (45))
+                                                                    (Prims.of_int (36)))))
+                                                                    (FStar_Sealed.seal
+                                                                    (Obj.magic
+                                                                    (FStar_Range.mk_range
+                                                                    "Pulse.Checker.Rewrite.fst"
+                                                                    (Prims.of_int (45))
+                                                                    Prims.int_one
+                                                                    (Prims.of_int (45))
+                                                                    (Prims.of_int (54)))))
+                                                                    (Obj.magic
+                                                                    (Pulse_Prover.try_frame_pre
+                                                                    g pre ()
+                                                                    (Pulse_Typing.wr
+                                                                    (Pulse_Syntax_Base.Tm_Rewrite
+                                                                    {
+                                                                    Pulse_Syntax_Base.t1
+                                                                    = p1;
+                                                                    Pulse_Syntax_Base.t2
+                                                                    = q1
+                                                                    }))
+                                                                    (Pulse_Typing.comp_rewrite
+                                                                    p1 q1) d))
+                                                                    (fun
+                                                                    uu___3 ->
+                                                                    (fun
+                                                                    uu___3 ->
+                                                                    Obj.magic
+                                                                    (Pulse_Prover.repack
+                                                                    g pre
+                                                                    uu___3
+                                                                    post_hint
+                                                                    t.Pulse_Syntax_Base.range2))
+                                                                    uu___3)))
+                                                                    uu___3)))
+                                                                    uu___3)))
+                                                            uu___2))) uu___1)))
+                              uu___))) uu___)
